theories/Spilling/RepairSpillSound.v
@@ -255,3 +255,4 @@ Proof.
         -- apply subset_cardinal;eauto. clear; cset_tac.
         -- rewrite subset_cardinal;eauto. clear; cset_tac.
   - admit.
+Admitted.
